Improve def of exp_sim & prove exp_sim cong for Lam

ctxt_equivScript.sml
@@ -1,7 +1,7 @@
 
 open HolKernel Parse boolLib bossLib term_tactic;
 open arithmeticTheory listTheory stringTheory alistTheory optionTheory
-     ltreeTheory llistTheory bagTheory pure_langTheory;
+     ltreeTheory llistTheory bagTheory pure_langTheory pairTheory pred_setTheory;
 
 
 val _ = new_theory "ctxt_equiv";
@@ -24,6 +24,7 @@ End
 
 Definition plug_def:
   plug Hole n = n ∧
+  plug (Prim op xs1 h xs2) n = Prim op (xs1 ++ [plug h n] ++ xs2) ∧
   plug (AppL h y) n = App (plug h n) y ∧
   plug (AppR x h) n = App x (plug h n) ∧
   plug (Lam v h) n = Lam v (plug h n) ∧
@@ -36,9 +37,8 @@ End
 
 Definition exp_sim_def:
   exp_sim c x y ⇔
-    set (freevars x) = set (freevars y) ∧
     ∀bindings.
-      set (MAP FST bindings) = set (freevars y) ⇒
+      set (freevars x) ∪ set (freevars y) ⊆ set (MAP FST bindings) ⇒
       exp_rel c (bind bindings x) (bind bindings y)
 End
 
@@ -47,12 +47,59 @@ Theorem exp_sim_closed:
   exp_sim c x y = exp_rel c x y
 Proof
   fs [closed_def,exp_sim_def,bind_def]
+  \\ rw [] \\ eq_tac \\ rw []
+  THEN1 (first_x_assum (qspec_then ‘[]’ mp_tac) \\ fs [bind_def])
+  \\ fs [GSYM closed_def]
+  \\ rpt (pop_assum mp_tac)
+  \\ qid_spec_tac ‘x’
+  \\ qid_spec_tac ‘y’
+  \\ qid_spec_tac ‘bindings’
+  \\ ho_match_mp_tac SNOC_INDUCT
+  \\ fs [bind_def] \\ rw []
+  \\ rewrite_tac [SNOC_APPEND,GSYM bind_bind,bind_def]
+  \\ rename [‘bind [t]’] \\ PairCases_on ‘t’ \\ fs [bind_def]
+  \\ reverse IF_CASES_TAC \\ fs [AND_IMP_INTRO]
+  \\ first_x_assum match_mp_tac \\ fs [exp_rel_def,v_rel_refl]
+  \\ EVAL_TAC
 QED
 
-Theorem exp_sim:
-  exp_sim c x y ⇒ exp_sim c (plug h x) (plug h y)
+Theorem bind_Lam:
+  ∀xs s x.
+    bind xs (Lam s x) =
+      if EVERY closed (MAP SND xs) then
+        Lam s (bind (FILTER (λy. FST y ≠ s) xs) x)
+      else Fail
 Proof
-  cheat (* help? *)
+  Induct \\ fs [bind_def,FORALL_PROD]
+  \\ rw [subst_def,bind_def] \\ fs []
+QED
+
+Theorem exp_sim_Lam:
+  exp_sim c x y ⇒ exp_sim c (Lam s x) (Lam s y)
+Proof
+  fs [exp_sim_def] \\ rw []
+  \\ fs [bind_Lam]
+  \\ rw [] \\ fs []
+  \\ fs [exp_rel_def,v_rel_refl,eval_Lam]
+  \\ fs [v_rel_def]
+  \\ Cases \\ fs [v_rel'_def]
+  \\ disj2_tac \\ rw []
+  \\ fs [PULL_FORALL,bind_bind]
+  \\ first_x_assum match_mp_tac
+  \\ fs [EXTENSION,MEM_MAP,MEM_FILTER,EXISTS_PROD,SUBSET_DEF]
+  \\ metis_tac []
+QED
+
+Theorem exp_sim_plug:
+  ∀h x y. exp_sim c x y ⇒ exp_sim c (plug h x) (plug h y)
+Proof
+  ho_match_mp_tac plug_ind \\ rw []
+  THEN1 (rename [‘Hole’] \\ fs [plug_def])
+  THEN1 (rename [‘Prim’] \\ cheat (* help? *))
+  THEN1 (rename [‘AppL’] \\ cheat (* help? *))
+  THEN1 (rename [‘AppR’] \\ cheat (* help? *))
+  THEN1 (rename [‘Lam’] \\ fs [plug_def,exp_sim_Lam])
+  \\ cheat (* help? *)
 QED
 
 val _ = export_theory();
